theory/Static_Communication_Analysis.thy
@@ -5,194 +5,200 @@ theory Static_Communication_Analysis
     Static_Framework
 begin
 
+type_synonym label_map = "node_label \<Rightarrow> var set"
 
-inductive built_on_chan :: "abstract_value_env \<Rightarrow> var \<Rightarrow> var \<Rightarrow> bool"  where
+inductive built_on_chan :: "abstract_value_env \<Rightarrow> label_map \<Rightarrow> var \<Rightarrow> var \<Rightarrow> bool"  where
   Chan: "
     \<lbrakk>
       ^Chan x\<^sub>c \<in> V x 
     \<rbrakk> \<Longrightarrow> 
-    built_on_chan V x\<^sub>c x
+    built_on_chan V Ln x\<^sub>c x
   " |
   Send_Evt: "
     \<lbrakk>
       ^Send_Evt x\<^sub>s\<^sub>c x\<^sub>m \<in> V x;
-      built_on_chan V x\<^sub>c x\<^sub>s\<^sub>c \<or> built_on_chan V x\<^sub>c x\<^sub>m 
+      built_on_chan V Ln x\<^sub>c x\<^sub>s\<^sub>c \<or> built_on_chan V Ln x\<^sub>c x\<^sub>m 
     \<rbrakk> \<Longrightarrow> 
-    built_on_chan V x\<^sub>c x
+    built_on_chan V Ln x\<^sub>c x
   " |
   Recv_Evt: "
     \<lbrakk>
       ^Recv_Evt x\<^sub>r\<^sub>c \<in> V x;
-      built_on_chan V x\<^sub>c x\<^sub>r\<^sub>c
+      built_on_chan V Ln x\<^sub>c x\<^sub>r\<^sub>c
     \<rbrakk> \<Longrightarrow> 
-    built_on_chan V x\<^sub>c x
+    built_on_chan V Ln x\<^sub>c x
   " |
   Pair: "
     \<lbrakk>
       ^(Pair x\<^sub>1 x\<^sub>2) \<in> V x;
-      built_on_chan V x\<^sub>c x\<^sub>1 \<or> built_on_chan V x\<^sub>c x\<^sub>2
+      built_on_chan V Ln x\<^sub>c x\<^sub>1 \<or> built_on_chan V Ln x\<^sub>c x\<^sub>2
     \<rbrakk> \<Longrightarrow> 
-    built_on_chan V x\<^sub>c x
+    built_on_chan V Ln x\<^sub>c x
   " |
   Left: "
     \<lbrakk>
       ^(Left x\<^sub>a) \<in> V x;
-      built_on_chan V x\<^sub>c x\<^sub>a
+      built_on_chan V Ln x\<^sub>c x\<^sub>a
     \<rbrakk> \<Longrightarrow> 
-    built_on_chan V x\<^sub>c x
+    built_on_chan V Ln x\<^sub>c x
   " |
   Right: "
     \<lbrakk>
       ^(Right x\<^sub>a) \<in> V x;
-      built_on_chan V x\<^sub>c x\<^sub>a
+      built_on_chan V Ln x\<^sub>c x\<^sub>a
     \<rbrakk> \<Longrightarrow> 
-    built_on_chan V x\<^sub>c x
+    built_on_chan V Ln x\<^sub>c x
+  " |
+  Abs: "
+    ^Abs f x\<^sub>p e\<^sub>b \<in> V x \<Longrightarrow> 
+    \<not> Set.is_empty (Ln (nodeLabel e\<^sub>b)) \<Longrightarrow>
+    built_on_chan V Ln x\<^sub>c x
   "
 
 
-fun chanSet :: "abstract_value_env \<Rightarrow> var \<Rightarrow> var \<Rightarrow> var set" where
-  "chanSet V x\<^sub>c x = (if built_on_chan V x\<^sub>c x then {x} else {})"
+fun chanSet :: "abstract_value_env \<Rightarrow> label_map \<Rightarrow> var \<Rightarrow> var \<Rightarrow> var set" where
+  "chanSet V Ln x\<^sub>c x = (if built_on_chan V Ln x\<^sub>c x then {x} else {})"
 
 
-type_synonym label_map = "node_label \<Rightarrow> var set"
+
+
+(*
+  need \<subseteq> instead of = for liveness sets, because variables are not necessarily unique.
+  also, additional values may be included in outer abstractions.
+*)
 inductive static_chan_liveness :: "abstract_value_env \<Rightarrow> label_map \<Rightarrow> label_map \<Rightarrow> var \<Rightarrow> exp \<Rightarrow> bool" where
   Result: "
     \<lbrakk>
-      chanSet V x\<^sub>c y \<subseteq> Ln (NResult y)
+      chanSet V Ln x\<^sub>c y \<subseteq> Ln (NResult y)
     \<rbrakk> \<Longrightarrow>
     static_chan_liveness V Ln Lx x\<^sub>c (RESULT y)
   " |
   Let_Unit: "
     \<lbrakk>
+      static_chan_liveness V Ln Lx x\<^sub>c e;
       Ln (nodeLabel e) \<subseteq> Lx (NLet x);
-      Lx (NLet x) \<subseteq> Ln (NLet x);
-      static_chan_liveness V Ln Lx x\<^sub>c e
+      Lx (NLet x) \<subseteq> Ln (NLet x)
     \<rbrakk> \<Longrightarrow>
     static_chan_liveness V Ln Lx x\<^sub>c (LET x = \<lparr>\<rparr> in e)
   " |
   Let_Chan: "
     \<lbrakk>
-      Ln (nodeLabel e) \<union> (chanSet V x\<^sub>c x) \<subseteq> Lx (NLet x);
-      (Lx (NLet x) - chanSet V x\<^sub>c x) \<subseteq> Ln (NLet x);
-      static_chan_liveness V Ln Lx x\<^sub>c e
+      static_chan_liveness V Ln Lx x\<^sub>c e;
+      Ln (nodeLabel e) \<subseteq> Lx (NLet x);
+      (Lx (NLet x) - {x}) \<subseteq> Ln (NLet x)
     \<rbrakk> \<Longrightarrow>
     static_chan_liveness V Ln Lx x\<^sub>c (LET x = CHAN \<lparr>\<rparr> in e)
   " |
   Let_Send_Evt: "
     \<lbrakk>
-      Ln (nodeLabel e) \<union> (chanSet V x\<^sub>c x) \<subseteq> Lx (NLet x);
-      (
-        (Lx (NLet x) - chanSet V x\<^sub>c x) \<union> 
-        chanSet V x\<^sub>c x\<^sub>s\<^sub>c \<union> chanSet V x\<^sub>c x\<^sub>m 
-      ) \<subseteq> Ln (NLet x);
-      static_chan_liveness V Ln Lx x\<^sub>c e
+      static_chan_liveness V Ln Lx x\<^sub>c e;
+      Ln (nodeLabel e) \<subseteq> Lx (NLet x);
+      (Lx (NLet x) - {x}) \<union> chanSet V Ln x\<^sub>c x\<^sub>s\<^sub>c \<union> chanSet V Ln x\<^sub>c x\<^sub>m \<subseteq> Ln (NLet x)
     \<rbrakk> \<Longrightarrow>
     static_chan_liveness V Ln Lx x\<^sub>c (LET x = SEND EVT x\<^sub>s\<^sub>c x\<^sub>m in e)
   " |
   Let_Recv_Evt: "
     \<lbrakk>
-      Ln (nodeLabel e) \<union> (chanSet V x\<^sub>c x) \<subseteq> Lx (NLet x);
-      (Lx (NLet x) - chanSet V x\<^sub>c x) \<union> chanSet V x\<^sub>c x\<^sub>r\<^sub>c \<subseteq> Ln (NLet x);
-      static_chan_liveness V Ln Lx x\<^sub>c e
+      static_chan_liveness V Ln Lx x\<^sub>c e;
+      Ln (nodeLabel e) \<subseteq> Lx (NLet x);
+      (Lx (NLet x) - {x}) \<union> chanSet V Ln x\<^sub>c x\<^sub>r\<^sub>c \<subseteq> Ln (NLet x)
     \<rbrakk> \<Longrightarrow>
     static_chan_liveness V Ln Lx x\<^sub>c (LET x = RECV EVT x\<^sub>r\<^sub>c in e)
   " |
   Let_Pair: "
     \<lbrakk>
-      Ln (nodeLabel e) \<union> (chanSet V x\<^sub>c x) \<subseteq> Lx (NLet x);
-      (
-        (Lx (NLet x) - chanSet V x\<^sub>c x) \<union> 
-        chanSet V x\<^sub>c x\<^sub>1 \<union> chanSet V x\<^sub>c x\<^sub>2
-      ) \<subseteq> Ln (NLet x);
-      static_chan_liveness V Ln Lx x\<^sub>c e
+      static_chan_liveness V Ln Lx x\<^sub>c e;
+      Ln (nodeLabel e) \<subseteq> Lx (NLet x);
+      (Lx (NLet x) - {x}) \<union>  chanSet V Ln x\<^sub>c x\<^sub>1 \<union> chanSet V Ln x\<^sub>c x\<^sub>2 \<subseteq> Ln (NLet x)
     \<rbrakk> \<Longrightarrow>
     static_chan_liveness V Ln Lx x\<^sub>c (LET x = \<lparr>x\<^sub>1, x\<^sub>2\<rparr> in e)
   " |
   Let_Left: "
     \<lbrakk>
-      Ln (nodeLabel e) \<union> (chanSet V x\<^sub>c x) \<subseteq> Lx (NLet x);
-      (Lx (NLet x) - chanSet V x\<^sub>c x) \<union> chanSet V x\<^sub>c x\<^sub>a \<subseteq> Ln (NLet x);
-      static_chan_liveness V Ln Lx x\<^sub>c e
+      static_chan_liveness V Ln Lx x\<^sub>c e;
+      Ln (nodeLabel e) \<subseteq> Lx (NLet x);
+      (Lx (NLet x) - {x}) \<union> chanSet V Ln x\<^sub>c x\<^sub>a \<subseteq> Ln (NLet x)
     \<rbrakk> \<Longrightarrow>
     static_chan_liveness V Ln Lx x\<^sub>c (LET x = LEFT x\<^sub>a in e)
   " |
   Let_Right: "
     \<lbrakk>
-      Ln (nodeLabel e) \<union> (chanSet V x\<^sub>c x) \<subseteq> Lx (NLet x);
-      (Lx (NLet x) - chanSet V x\<^sub>c x) \<union> chanSet V x\<^sub>c x\<^sub>a \<subseteq> Ln (NLet x);
-      static_chan_liveness V Ln Lx x\<^sub>c e
+      static_chan_liveness V Ln Lx x\<^sub>c e;
+      Ln (nodeLabel e) \<subseteq> Lx (NLet x);
+      (Lx (NLet x) - {x}) \<union> chanSet V Ln x\<^sub>c x\<^sub>a \<subseteq> Ln (NLet x)
     \<rbrakk> \<Longrightarrow>
     static_chan_liveness V Ln Lx x\<^sub>c (LET x = RIGHT x\<^sub>a in e)
   " |
   Let_Abs: "
     \<lbrakk>
-      Ln (nodeLabel e) \<union> (chanSet V x\<^sub>c x) \<subseteq> Lx (NLet x);
-      (Lx (NLet x) - chanSet V x\<^sub>c x) \<subseteq> Ln (NLet x);
+
+      static_chan_liveness V Ln Lx x\<^sub>c e;
+      Ln (nodeLabel e) \<subseteq> Lx (NLet x);
       static_chan_liveness V Ln Lx x\<^sub>c e\<^sub>b;
-      static_chan_liveness V Ln Lx x\<^sub>c e
+      (Lx (NLet x) - {x}) \<union> Ln (nodeLabel e\<^sub>b) \<subseteq> Ln (NLet x)
     \<rbrakk> \<Longrightarrow>
     static_chan_liveness V Ln Lx x\<^sub>c (LET x = FN f x\<^sub>p . e\<^sub>b  in e)
   " |
   Let_Spawn: "
     \<lbrakk>
-      Ln (nodeLabel e) \<union> (chanSet V x\<^sub>c x) \<subseteq> Lx (NLet x);
-      (Lx (NLet x) - chanSet V x\<^sub>c x) \<subseteq> Ln (NLet x);
+      static_chan_liveness V Ln Lx x\<^sub>c e;
       static_chan_liveness V Ln Lx x\<^sub>c e\<^sub>c;
-      static_chan_liveness V Ln Lx x\<^sub>c e
+      Ln (nodeLabel e) \<union> Ln (nodeLabel e\<^sub>c) \<subseteq> Lx (NLet x);
+      (Lx (NLet x) - {x}) \<subseteq> Ln (NLet x)
     \<rbrakk> \<Longrightarrow>
     static_chan_liveness V Ln Lx x\<^sub>c (LET x = SPAWN e\<^sub>c in e)
   " |
   Let_Sync: "
     \<lbrakk>
-      Ln (nodeLabel e) \<union> (chanSet V x\<^sub>c x) \<subseteq> Lx (NLet x);
-      \<forall> xSC xM . {^Send_Evt xSC xM} \<subseteq> V x\<^sub>e \<longrightarrow> (chanSet V x\<^sub>c xM) \<subseteq> Lx (NLet x);
-      (Lx (NLet x) - chanSet V x\<^sub>c x) \<union> chanSet V x\<^sub>c x\<^sub>e \<subseteq> Ln (NLet x);
-      static_chan_liveness V Ln Lx x\<^sub>c e
+      static_chan_liveness V Ln Lx x\<^sub>c e;
+      Ln (nodeLabel e) \<subseteq> Lx (NLet x);
+      (Lx (NLet x) - {x}) \<union> chanSet V Ln x\<^sub>c x\<^sub>e \<subseteq> Ln (NLet x)
     \<rbrakk> \<Longrightarrow>
     static_chan_liveness V Ln Lx x\<^sub>c (LET x = SYNC x\<^sub>e in e)
   " |
   Let_Fst: "
     \<lbrakk>
-      Ln (nodeLabel e) \<union> (chanSet V x\<^sub>c x) \<subseteq> Lx (NLet x);
-      (Lx (NLet x) - chanSet V x\<^sub>c x) \<union> chanSet V x\<^sub>c x\<^sub>a \<subseteq> Ln (NLet x);
-      static_chan_liveness V Ln Lx x\<^sub>c e
+      static_chan_liveness V Ln Lx x\<^sub>c e;
+      Ln (nodeLabel e) \<subseteq> Lx (NLet x);
+      (Lx (NLet x) - {x}) \<union> chanSet V Ln x\<^sub>c x\<^sub>a \<subseteq> Ln (NLet x)
     \<rbrakk> \<Longrightarrow>
     static_chan_liveness V Ln Lx x\<^sub>c (LET x = FST x\<^sub>a in e)
   " |
   Let_Snd: "
     \<lbrakk>
-      Ln (nodeLabel e) \<union> (chanSet V x\<^sub>c x) \<subseteq> Lx (NLet x);
-      (Lx (NLet x) - chanSet V x\<^sub>c x) \<union> chanSet V x\<^sub>c x\<^sub>a \<subseteq> Ln (NLet x);
-      static_chan_liveness V Ln Lx x\<^sub>c e
+      static_chan_liveness V Ln Lx x\<^sub>c e;
+      Ln (nodeLabel e) \<subseteq> Lx (NLet x);
+      (Lx (NLet x) - {x}) \<union> chanSet V Ln x\<^sub>c x\<^sub>a \<subseteq> Ln (NLet x)
     \<rbrakk> \<Longrightarrow>
     static_chan_liveness V Ln Lx x\<^sub>c (LET x = SND x\<^sub>a in e)
   " |
   Let_Case: "
     \<lbrakk>
-      Ln (nodeLabel e\<^sub>l) \<union> Ln (nodeLabel e\<^sub>r) \<union> (chanSet V x\<^sub>c x) \<subseteq> Lx (NLet x);
-      (Lx (NLet x) - chanSet V x\<^sub>c x) \<union> chanSet V x\<^sub>c x\<^sub>s \<subseteq> Ln (NLet x);
-
-      Ln (nodeLabel e) \<subseteq> Lx (NResult (\<lfloor>e\<^sub>l\<rfloor>));
-      Lx (NResult (\<lfloor>e\<^sub>l\<rfloor>)) \<union> chanSet V x\<^sub>c (\<lfloor>e\<^sub>l\<rfloor>) \<subseteq> Ln (NResult (\<lfloor>e\<^sub>l\<rfloor>));
-
+      static_chan_liveness V Ln Lx x\<^sub>c e;
       Ln (nodeLabel e) \<subseteq> Lx (NResult (\<lfloor>e\<^sub>r\<rfloor>));
-      Lx (NResult (\<lfloor>e\<^sub>r\<rfloor>)) \<union> chanSet V x\<^sub>c (\<lfloor>e\<^sub>r\<rfloor>) \<subseteq> Ln (NResult (\<lfloor>e\<^sub>r\<rfloor>));
+      Ln (nodeLabel e) \<subseteq> Lx (NResult (\<lfloor>e\<^sub>l\<rfloor>));
+
+      Lx (NResult (\<lfloor>e\<^sub>r\<rfloor>)) \<union> chanSet V Ln x\<^sub>c (\<lfloor>e\<^sub>r\<rfloor>) \<subseteq> Ln (NResult (\<lfloor>e\<^sub>r\<rfloor>));
+      Lx (NResult (\<lfloor>e\<^sub>l\<rfloor>)) \<union> chanSet V Ln x\<^sub>c (\<lfloor>e\<^sub>l\<rfloor>) \<subseteq> Ln (NResult (\<lfloor>e\<^sub>l\<rfloor>));
 
       static_chan_liveness V Ln Lx x\<^sub>c e\<^sub>l;
       static_chan_liveness V Ln Lx x\<^sub>c e\<^sub>r;
-      static_chan_liveness V Ln Lx x\<^sub>c e
+      Ln (nodeLabel e\<^sub>l) \<union> Ln (nodeLabel e\<^sub>r) \<subseteq> Lx (NLet x);
+      (Lx (NLet x) - {x}) \<union> chanSet V Ln x\<^sub>c x\<^sub>s \<subseteq> Ln (NLet x)
+
     \<rbrakk> \<Longrightarrow>
     static_chan_liveness V Ln Lx x\<^sub>c (LET x = CASE x\<^sub>s LEFT x\<^sub>l |> e\<^sub>l RIGHT x\<^sub>r |> e\<^sub>r in e)
   " |
   Let_App: "
     \<lbrakk>
+      static_chan_liveness V Ln Lx x\<^sub>c e;
       (\<forall> f' x\<^sub>p e\<^sub>b . ^Abs f' x\<^sub>p e\<^sub>b \<in> V f \<longrightarrow> 
         Ln (nodeLabel e) \<subseteq> Lx (NResult (\<lfloor>e\<^sub>b\<rfloor>)) \<and>
-        Lx (NResult (\<lfloor>e\<^sub>b\<rfloor>)) \<union> chanSet V x\<^sub>c (\<lfloor>e\<^sub>b\<rfloor>) \<subseteq> Ln (NResult (\<lfloor>e\<^sub>b\<rfloor>)) \<and>
-        Ln (nodeLabel e\<^sub>b) \<union> (chanSet V x\<^sub>c x) \<subseteq> Lx (NLet x)
+        Lx (NResult (\<lfloor>e\<^sub>b\<rfloor>)) \<union> chanSet V Ln x\<^sub>c (\<lfloor>e\<^sub>b\<rfloor>) \<subseteq> Ln (NResult (\<lfloor>e\<^sub>b\<rfloor>)) \<and>
+        Ln (nodeLabel e\<^sub>b) \<subseteq> Lx (NLet x)
       );
-      (Lx (NLet x) - chanSet V x\<^sub>c x) \<union> chanSet V x\<^sub>c x\<^sub>a \<subseteq> Ln (NLet x);
-      static_chan_liveness V Ln Lx x\<^sub>c e
+      (Lx (NLet x) - {x}) \<union> chanSet V Ln x\<^sub>c x\<^sub>a \<subseteq> Ln (NLet x)
+
     \<rbrakk> \<Longrightarrow>
     static_chan_liveness V Ln Lx x\<^sub>c (LET x = APP f x\<^sub>a in e)
   "
@@ -209,25 +215,24 @@ inductive is_static_live_flow :: "label_map \<Rightarrow> label_map \<Rightarrow
     (l, ENext, l') \<in> F \<Longrightarrow>
     \<not> Set.is_empty (Lx l) \<Longrightarrow>
     \<not> Set.is_empty (Ln l') \<Longrightarrow>
-    is_static_live_flow Ln Lx F (l, ENext, l')
+    is_static_live_flow Ln Lx F (l, ESpawn, l')
   " |
   Call: "
     (l, ENext, l') \<in> F \<Longrightarrow>
     \<not> Set.is_empty (Lx l) \<Longrightarrow>
     \<not> Set.is_empty (Ln l') \<Longrightarrow>
-    is_static_live_flow Ln Lx F (l, ENext, l')
+    is_static_live_flow Ln Lx F (l, ECall, l')
   " |
   Return: "
     (l, ENext, l') \<in> F \<Longrightarrow>
     \<not> Set.is_empty (Lx l) \<Longrightarrow>
     \<not> Set.is_empty (Ln l') \<Longrightarrow>
-    is_static_live_flow Ln Lx F (l, ENext, l')
+    is_static_live_flow Ln Lx F (l, EReturn, l')
   " |
   Send: "
-    ((NLet xSend), ESend, (NLet xRecv)) \<in> F \<Longrightarrow>
-    \<not> Set.is_empty (Lx (NLet xSend)) \<Longrightarrow>
-    {xRecv} \<subseteq> (Ln (NLet xRecv)) \<Longrightarrow>
-    is_static_live_flow Ln Lx F ((NLet xSend), ESend, (NLet xRecv))
+    ((NLet xSend), ESend xM, (NLet xRecv)) \<in> F \<Longrightarrow>
+    {xM} \<subseteq> (Ln (NLet xSend)) \<Longrightarrow>
+    is_static_live_flow Ln Lx F ((NLet xSend), ESend xM, (NLet xRecv))
   "
 
 
@@ -287,10 +292,10 @@ inductive inclusive :: "static_path \<Rightarrow> static_path \<Rightarrow> bool
     \<pi> @ (NLet x, ENext) # \<pi>\<^sub>1 \<asymp> \<pi> @ (NLet x, ESpawn) # \<pi>\<^sub>2
   " |
   Send_Left: "
-    \<pi> @ (NLet x, ESend) # \<pi>\<^sub>1 \<asymp> \<pi> @ (NLet x, ENext) # \<pi>\<^sub>2
+    \<pi> @ (NLet x, ESend xM) # \<pi>\<^sub>1 \<asymp> \<pi> @ (NLet x, ENext) # \<pi>\<^sub>2
   " |
   Send_Right: "
-    \<pi> @ (NLet x, ENext) # \<pi>\<^sub>1 \<asymp> \<pi> @ (NLet x, ESend) # \<pi>\<^sub>2
+    \<pi> @ (NLet x, ENext) # \<pi>\<^sub>1 \<asymp> \<pi> @ (NLet x, ESend xM) # \<pi>\<^sub>2
   "
 
 lemma inclusive_commut: "
